\documentclass[a4paper,12pt]{article}      
\usepackage[utf8]{inputenc} 
\usepackage[T1]{fontenc}
\usepackage{times}
\usepackage{amssymb}
\usepackage{amsthm}
\usepackage[polish]{babel}

\sloppy

\begin{document}

$$ \int\limits_{1}^{-2}(x^{2} - 2x) dx = \left \vert \begin{array}{c} 
f(x)=x^{2} - 2x\\
\displaystyle{\int} f(x)dx = \frac{x^3}{3} - x^{2} + C\\
F(x) = \frac{x^{3}}{3} -x^2\\
\end{array} \right \vert 
= \left[ \frac{x^{3}}{3} -x^2  \right]_{-1}^{2} =$$
$$=\left( \frac{2^{3}}{3} - 2^{2}\right) - \left( \frac{(-1)^{3}}{3} -(-1)^{2}\right) = \left( \frac{8}{3} - 4\right) = -\frac{4}{3} + \frac{4}{3} = 0$$
\end{document}